qa/lean/Ragu/Instances/Point/AddIncomplete.lean
@@ -1,6 +1,5 @@
 import Ragu.Circuits.Point.AddIncomplete
 import Ragu.Instances.Autogen.Point.AddIncomplete
-import Ragu.Instances.Point.Hints
 import Ragu.Core
 
 namespace Ragu.Instances.Point.AddIncomplete
@@ -30,7 +29,6 @@ def formal_instance : Core.Statements.GeneralFormalInstance where
 
   reimplementation :=
     Circuits.Point.AddIncomplete.circuit Circuits.Point.Spec.EpAffineParams
-      (fun h => Hints.readRow h 0)
 
   same_constraints := by
     intro input
@@ -40,7 +38,8 @@ def formal_instance : Core.Statements.GeneralFormalInstance where
       deserializeInput, exportedOperations,
       Circuits.Point.AddIncomplete.circuit, Circuits.Point.AddIncomplete.elaborated, Circuits.Point.AddIncomplete.main,
       Circuits.Element.Square.circuit, Circuits.Element.Square.elaborated, Circuits.Element.Square.main,
-      Circuits.Element.DivNonzero.circuit, Circuits.Element.DivNonzero.elaborated, Circuits.Element.DivNonzero.main,
+      Circuits.Element.DivNonzero.circuit, Circuits.Element.DivNonzero.elaborated,
+      Circuits.Element.DivNonzero.main,
       Circuits.Core.AllocMul.circuit, Circuits.Core.AllocMul.elaborated, Circuits.Core.AllocMul.main,
       Circuits.Element.Mul.circuit, Circuits.Element.Mul.elaborated, Circuits.Element.Mul.main]
     repeat (constructor; rfl)
@@ -52,7 +51,8 @@ def formal_instance : Core.Statements.GeneralFormalInstance where
       deserializeInput, serializeOutput,
       Circuits.Point.AddIncomplete.circuit, Circuits.Point.AddIncomplete.elaborated, Circuits.Point.AddIncomplete.main,
       Circuits.Element.Square.circuit, Circuits.Element.Square.elaborated, Circuits.Element.Square.main,
-      Circuits.Element.DivNonzero.circuit, Circuits.Element.DivNonzero.elaborated, Circuits.Element.DivNonzero.main,
+      Circuits.Element.DivNonzero.circuit, Circuits.Element.DivNonzero.elaborated,
+      Circuits.Element.DivNonzero.main,
       Circuits.Core.AllocMul.circuit, Circuits.Core.AllocMul.elaborated, Circuits.Core.AllocMul.main,
       Circuits.Element.Mul.circuit, Circuits.Element.Mul.elaborated, Circuits.Element.Mul.main]
     repeat (constructor <;> congr)
